Updated langauge.rs and made enums more explicit in coq backend

language/tests/language.rs
@@ -1,7 +1,8 @@
 use assert_cmd::prelude::*; // Add methods on commands
+use std::collections::HashMap;
 use std::{env, process::Command};
 
-fn run_test(file_name: &str, output: Option<&str>) {
+fn run_test_option(file_name: &str, output: Option<&str>) {
     let mut cmd = Command::cargo_bin("cargo-hacspec").expect("Error getting cargo hacspec command");
     cmd.envs(env::vars());
     if let Some(f) = output {
@@ -15,32 +16,63 @@ fn run_test(file_name: &str, output: Option<&str>) {
     assert!(status.success());
 }
 
+fn run_test(file_name: &str) {
+    run_test_option(file_name, None);
+}
+
+fn run_test_with_output(file_name: &str, output: &str) {
+    run_test_option(file_name, Some(output));
+}
+
+fn run_tests(file_name: &str, output_name: &str, output: HashMap<&str, bool>) {
+    let hacspec_targets = vec![("fstar", "tests/", ".fst"), ("coq", "tests/coq/", ".v")];
+
+    hacspec_targets.iter().fold((), |(), (name, pre, post)| {
+        if output.contains_key(name) && output[name] {
+            run_test_with_output(file_name, (pre.to_string() + output_name + post).as_str());
+        }
+    });
+}
+
 #[test]
 fn positive_question_mark() {
-    run_test(
+    run_tests(
         "language-tests/question_mark.rs",
-        Some("tests/QuestionMark.fst"),
+        "QuestionMark",
+        HashMap::from([("fstar", true), ("coq", true)]),
     );
 }
 
 #[test]
 fn positive_result() {
-    run_test("language-tests/result.rs", Some("tests/Result.fst"));
+    run_tests(
+        "language-tests/result.rs",
+        "Result",
+        HashMap::from([("fstar", true), ("coq", true)]),
+    );
 }
 
 #[test]
 fn positive_enums() {
-    run_test("language-tests/enums.rs", Some("tests/Enums.fst"));
+    run_tests(
+        "language-tests/enums.rs",
+        "Enums",
+        HashMap::from([("fstar", true), ("coq", true)]),
+    );
 }
 
 #[test]
 fn positive_option() {
-    run_test("language-tests/option.rs", Some("tests/Option.fst"));
+    run_tests(
+        "language-tests/option.rs",
+        "Option",
+        HashMap::from([("fstar", true), ("coq", true)]),
+    );
 }
 
 #[test]
 fn positive_arrays() {
-    run_test("language-tests/arrays.rs", None);
+    run_test("language-tests/arrays.rs");
 }
 
 #[test]
@@ -50,26 +82,28 @@ fn positive_copy() {
 
 #[test]
 fn positive_tuples() {
-    run_test("language-tests/tuples.rs", None);
+    run_test("language-tests/tuples.rs");
 }
 
 #[test]
 fn positive_loops() {
-    run_test("language-tests/loops.rs", None);
+    run_tests("language-tests/loops.rs",
+              "Loops",
+              HashMap::from([("coq", true)]));
 }
 
 #[test]
 fn positive_expr_block() {
-    run_test("language-tests/expr_block.rs", None);
+    run_test("language-tests/expr_block.rs");
 }
 
 #[test]
 fn positive_seq_ops() {
-    run_test("language-tests/seq_ops.rs", None);
+    run_test("language-tests/seq_ops.rs");
 }
 
 #[test]
 #[should_panic]
 fn negative_arrays() {
-    run_test("negative-language-tests/arrays.rs", None);
+    run_test("negative-language-tests/arrays.rs");
 }
